elo-coq/Properties2.v
@@ -1,0 +1,395 @@
+From Coq Require Import Arith.Arith.
+From Coq Require Import Lists.List.
+
+From Elo Require Export Array.
+From Elo Require Export Map.
+From Elo Require Export Core.
+
+Ltac splits n :=
+  match n with
+  | O => fail
+  | S O => idtac
+  | S ?n' => split; [| splits n']
+  end.
+
+(* ------------------------------------------------------------------------- *)
+(* Determinism ------------------------------------------------------------- *)
+(* ------------------------------------------------------------------------- *)
+
+Lemma value_does_not_step : forall v t eff,
+  value v -> ~ (v --> t # eff).
+Proof.
+  intros * Hv Hstep. destruct Hv; inversion Hstep.
+Qed.
+
+Theorem deterministic_step : forall t t1 t2 eff,
+  t --> t1 # eff ->
+  t --> t2 # eff ->
+  t1 = t2.
+Proof.
+  intros * Hstep1. generalize dependent t2.
+  induction Hstep1; intros * Hstep2; inversion Hstep2; subst;
+  try solve
+    [ congruence
+    | match goal with
+      | Hstep : ?v --> _ # _ , Hv : value ?v |- _ =>
+          eapply value_does_not_step in Hstep; eauto; contradiction
+      | F : TM_Nil         --> _ # _ |- _ => inversion F
+      | F : TM_Num _       --> _ # _ |- _ => inversion F
+      | F : TM_Arr _ _     --> _ # _ |- _ => inversion F
+      | F : TM_Fun _ _ _ _ --> _ # _ |- _ => inversion F
+      | F : TM_Loc _       --> _ # _ |- _ => inversion F
+      | H : forall x, _ --> x # _ -> _ = x |- _ => erewrite H; eauto
+      end
+    ].
+Qed.
+
+Theorem deterministic_typing : forall mt Gamma t X Y,
+  mt / Gamma |-- t is X ->
+  mt / Gamma |-- t is Y ->
+  X = Y.
+Proof.
+  intros * HX. generalize dependent Y.
+  induction HX; intros Y HY; inversion HY; subst;
+  try solve 
+    [ congruence
+    | auto
+    | match goal with
+      | IH : forall T, ?mt / ?Gamma |-- ?t is T -> (_ _) = T,
+        H : ?mt / ?Gamma |-- ?t is (_ _)
+        |- _ = _ => apply IH in H; congruence
+      end
+    ].
+Qed.
+
+(* ------------------------------------------------------------------------- *)
+(* Definitions ------------------------------------------------------------- *)
+(* ------------------------------------------------------------------------- *)
+
+Definition well_typed_memory mt m :=
+  length mt = length m /\
+  (forall i, mt / empty |-- (get_tm m i) is (get_typ mt i)).
+
+Definition well_typed_threads mt ths := forall i,
+  exists T, mt / empty |-- (get_tm ths i) is T.
+
+Definition well_typed_program mt m ths :=
+  well_typed_memory mt m /\
+  well_typed_threads mt ths.
+
+Definition finished ths :=
+  forall i, value (get_tm ths i).
+
+Inductive extends' {A} : list A -> list A -> Prop :=
+  | extends_nil : forall mt,
+    extends' mt nil
+  | extends_cons : forall x mt mt',
+    extends' mt mt' ->
+    extends' (x :: mt) (x :: mt').
+
+Infix "extends" := extends' (at level 50, left associativity).
+
+(* ------------------------------------------------------------------------- *)
+(* Auxiliary Lemmas -------------------------------------------------------- *)
+(* ------------------------------------------------------------------------- *)
+
+Lemma extends_refl : forall {A} (mt : list A),
+  mt extends mt.
+Proof.
+  induction mt; auto using @extends'.
+Qed.
+
+Lemma extends_add : forall {A} (mt : list A) a,
+  (add mt a) extends mt.
+Proof.
+  induction mt; eauto using @extends'.
+Qed.
+
+Lemma extends_length : forall {A} (mt mt' : list A) i,
+  i < length mt' ->
+  mt extends mt' ->
+  i < length mt.
+Proof.
+  intros *. generalize dependent mt. generalize dependent i.
+  induction mt'; intros * Hlen Hext.
+  - inversion Hlen.
+  - inversion Hext. destruct i;
+    eauto using PeanoNat.Nat.lt_0_succ, Lt.lt_n_S, Lt.lt_S_n.
+Qed.
+
+Lemma extends_lookup : forall (mt mt' : list typ) i,
+  i < length mt' ->
+  mt extends mt' ->
+  get_typ mt' i = get_typ mt i.
+Proof.
+  intros *. generalize dependent mt. generalize dependent i.
+  induction mt'; intros * Hlen Hext.
+  - inversion Hlen.
+  - inversion Hext. subst. destruct i.
+    + reflexivity.
+    + unfold get_typ, get. simpl in *. eauto using Lt.lt_S_n.
+Qed.
+
+Lemma safe_preserves_inclusion : forall Gamma Gamma',
+  Gamma includes Gamma' ->
+  (safe Gamma) includes (safe Gamma').
+Proof.
+  unfold Map.includes', safe. intros * H *.
+  destruct (Gamma k) eqn:E1; destruct (Gamma' k) eqn:E2;
+  solve [ intros F; inversion F
+        | eapply H in E2; rewrite E1 in E2; inversion E2; subst; trivial
+        ].
+Qed.
+
+Lemma update_safe_includes_comm : forall Gamma id T,
+  (update (safe Gamma) id T) includes (safe (update Gamma id T)).
+Proof.
+  unfold Map.includes', update, Map.update', safe. intros *.
+  destruct String.eqb; trivial.
+  destruct is_safe_type; trivial.
+  intros F. inversion F.
+Qed.
+
+Lemma memory_weakening : forall mt mt' Gamma t T, 
+  mt extends mt' ->
+  mt' / Gamma |-- t is T ->  
+  mt  / Gamma |-- t is T.
+Proof.
+  intros * Hext Htype.
+  induction Htype; eauto using @typeof, extends_length;
+  subst; erewrite extends_lookup; eauto using extends_length, @typeof.
+Qed.
+
+Lemma context_weakening : forall mt Gamma Gamma' t T,
+  Gamma includes Gamma' ->
+  mt / Gamma' |-- t is T ->
+  mt / Gamma  |-- t is T.
+Proof.
+  intros * Hinc Htype.
+  generalize dependent Gamma.
+  induction Htype; intros * Hinc;
+  eauto 6 using @typeof, safe_preserves_inclusion, update_preserves_inclusion.
+Qed.
+
+Lemma context_weakening_empty : forall mt Gamma t T,
+  mt / empty |-- t is T ->
+  mt / Gamma |-- t is T.
+Proof.
+  intros * Htype.
+  eapply (context_weakening _ _ empty); auto.
+  discriminate.
+Qed.
+
+Lemma substitution_preserves_typing : forall mt Gamma id t u T U,
+  mt / (update Gamma id U) |-- t is T ->
+  mt / empty |-- u is U ->
+  mt / Gamma |-- [id := u] t is T.
+Proof with eauto using context_weakening, context_weakening_empty,
+  lookup_update_kneq, update_overwrite, update_permutation,
+  update_safe_includes_comm.
+
+  intros * Ht Hu.
+  generalize dependent T. generalize dependent Gamma.
+  induction t; intros * Ht; inversion Ht; simpl; subst;
+  eauto using @typeof;
+  try (destruct String.eqb eqn:E);
+  try (apply String.eqb_eq in E; subst);
+  try (apply String.eqb_neq in E).
+  - rewrite lookup_update_keq in H1. inversion H1. subst...
+  - apply T_Id_Val. rewrite <- H1. symmetry...
+  - rewrite lookup_update_keq in H1. inversion H1. subst...
+  - apply T_Id_Var. rewrite <- H1. symmetry...
+  - eapply T_Spawn...
+  - apply T_LetVal...
+  - apply T_LetVal...
+  - apply T_LetVar...
+  - apply T_LetVar...
+  - eapply T_LetFun...
+  - eapply T_LetFun...
+  - apply T_Fun...
+  - apply T_Fun...
+Qed.
+
+Lemma stored_value_has_type : forall mt t t' addr v T,
+  t --> t' # EF_Store addr v ->
+  mt / empty |-- t is T ->
+  mt / empty |-- v is get_typ mt addr.
+Proof.
+  intros * Hstep Htype. generalize dependent t'.
+  induction Htype; intros * Hstep;
+  inversion Hstep; subst; eauto.
+  inversion Htype1. subst. eauto.
+Qed.
+
+Lemma spawn_block_has_type : forall mt t t' block T,
+  mt / empty |-- t is T ->
+  t --> t' # EF_Spawn block ->
+  exists B, mt / empty |-- block is B.
+Proof.
+  remember empty as Gamma.
+  intros * Htype. generalize dependent t'.
+  induction Htype; intros * Hstep; inversion Hstep; subst; eauto.
+Qed.
+
+Lemma set_preserves_memory_typing : forall m mt t i,
+  i < length m ->
+  well_typed_memory mt m ->
+  mt / empty |-- t is (get_typ mt i) ->
+  well_typed_memory mt (set m i t).
+Proof.
+  intros * ? [Hlen ?] ?. split.
+  - rewrite Hlen. apply set_preserves_length.
+  - intros j. destruct (i =? j) eqn:E.
+    + apply Nat.eqb_eq in E. subst. erewrite (get_set_involutive TM_Nil); auto.
+    + apply Nat.eqb_neq in E. erewrite (get_set_i_neq_j TM_Nil); auto.
+Qed.
+
+Lemma add_preserves_memory_typing : forall mt m t T,
+  well_typed_memory mt m ->
+  mt / empty |-- t is T ->
+  well_typed_memory (add mt T) (add m t).
+Proof.
+  intros * [Hlen Hmem] Htype.
+  split; auto using add_preserves_length. intros i.
+  destruct (lt_eq_lt_dec i (length m)) as [[Hlt | Heq] | Hgt];
+  unfold get_tm, get_typ in *; subst.
+  - rewrite get_add_lt; trivial.
+    rewrite <- Hlen in Hlt.
+    rewrite get_add_lt; trivial.
+    eauto using extends_add, memory_weakening.
+  - rewrite get_add_last. rewrite <- Hlen. rewrite get_add_last.
+    eauto using extends_add, memory_weakening.
+  - rewrite get_add_gt; trivial.
+    rewrite <- Hlen in Hgt.
+    rewrite get_add_gt; trivial.
+    apply T_Nil.
+Qed.
+
+Lemma set_preserves_thread_typing : forall mt ths t T i,
+  i < length ths ->
+  well_typed_threads mt ths ->
+  mt / empty |-- t is T ->
+  well_typed_threads mt (set ths i t).
+Proof.
+  intros * Hlen Htype Hstep.
+  intros i'. destruct (i =? i') eqn:E.
+  - apply Nat.eqb_eq in E. subst.
+    rewrite (get_set_involutive TM_Nil); eauto.
+  - apply Nat.eqb_neq in E. apply not_eq_sym in E.
+    rewrite (get_set_i_neq_j TM_Nil); eauto.
+Qed.
+
+Lemma add_preserves_thread_typing : forall mt ths t T,
+  well_typed_threads mt ths ->
+  mt / empty |-- t is T ->
+  well_typed_threads mt (add ths t).
+Proof.
+  intros * Hths Htype.
+  intros i. destruct (lt_eq_lt_dec i (length ths)) as [[? | Heq] | Hlt].
+  - specialize (Hths i) as [? ?]. rewrite (get_add_lt TM_Nil); eauto.
+  - subst. rewrite (get_add_last TM_Nil). eauto.
+  - rewrite (get_add_gt TM_Nil); eauto using T_Nil.
+Qed.
+
+(* ------------------------------------------------------------------------- *)
+(* Preservation ------------------------------------------------------------ *)
+(* ------------------------------------------------------------------------- *)
+
+Theorem limited_preservation : forall mt t t' eff T,
+  mt / empty |-- t is T ->
+  t --> t' # eff ->
+  ~ (exists addr v, EF_Load addr v = eff) ->
+  mt / empty |-- t' is T.
+Proof.
+  remember empty as Gamma.
+  intros * Htype Hstep Heff. generalize dependent t'.
+  induction Htype; intros * Hstep;
+  inversion Hstep; subst; eauto using @typeof, substitution_preserves_typing;
+  solve [contradiction Heff; eexists; eexists; eauto].
+Qed.
+
+Theorem preservation : forall ths ths' m m' mt,
+  well_typed_program mt m ths ->
+  m / ths ==> m' / ths' ->
+  exists mt',
+    mt' extends mt /\
+    well_typed_program mt' m' ths'.
+Proof.
+  intros * [Hmem Hths] Hcstep. induction Hcstep.
+  - exists mt. splits 3; eauto using extends_refl.
+    intros i'. destruct (i =? i') eqn:E.
+    + apply Nat.eqb_eq in E. subst.
+      rewrite (get_set_involutive TM_Nil); trivial.
+      specialize (Hths i') as [? ?]. eexists.
+      eapply limited_preservation; eauto. intros [? [? F]]. discriminate F.
+    + apply Nat.eqb_neq in E. apply not_eq_sym in E.
+      rewrite (get_set_i_neq_j TM_Nil); trivial.
+  - exists mt. splits 3; eauto using extends_refl.
+    intros i'. destruct (i =? i') eqn:E.
+    + apply Nat.eqb_eq in E. subst.
+      rewrite (get_set_involutive TM_Nil); trivial.
+      specialize Hmem as [? ?]. eexists. eauto.
+    + apply Nat.eqb_neq in E. apply not_eq_sym in E.
+      rewrite (get_set_i_neq_j TM_Nil); trivial.
+  - exists mt. splits 3; eauto using extends_refl.
+    + specialize (Hths i) as [T Htype].
+      apply set_preserves_memory_typing; eauto.
+      eauto using stored_value_has_type.
+    + destruct (Hths i) as [? ?].
+      eapply set_preserves_thread_typing; eauto.
+      eapply limited_preservation; eauto.
+      intros [? [? F]]. inversion F.
+  - eexists. splits 3; eauto using extends_refl.
+    destruct (Hths i) as [? ?].
+    assert (exists B, mt / empty |-- block is B) as [? Htype].
+    { eauto using spawn_block_has_type. }
+    eapply add_preserves_thread_typing; eauto. clear Htype.
+    eapply set_preserves_thread_typing; eauto.
+    eapply limited_preservation; eauto.
+    intros [? [? F]]. inversion F.
+Qed.
+
+(* ------------------------------------------------------------------------- *)
+(* Progress ---------------------------------------------------------------- *)
+(* ------------------------------------------------------------------------- *)
+
+Theorem limited_progress : forall m mt t T,
+  mt / empty |-- t is T ->
+  well_typed_memory mt m ->
+  (value t \/ exists t' eff, t --> t' # eff).
+Proof.
+  remember empty as Gamma. intros * Htype [Hlen Hmem].
+  assert (forall i, i < length mt -> i < length m). { rewrite Hlen. trivial. }
+  induction Htype; subst; auto using value; right;
+  try match goal with F : lookup empty _ = Some _ |- _ => inversion F end;
+  repeat match goal with
+    IH : _ = empty -> _ |- _ => specialize (IH eq_refl) as [? | [? [? ?]]]
+  end.
+  - eexists. eexists. eapplyeauto using step.
+  try solve [eexists; eexists; eauto using step];
+  repeat match goal with
+    Hv : value ?t , Htype : _ / _ |-- ?t is _ |- _ =>
+      destruct Hv; inversion Htype; subst
+  end;
+  eexists; eexists; eauto using step, value.
+Qed.
+
+Theorem progress : forall m mt ths,
+  well_typed_program mt m ths ->
+  (finished ths \/ exists m' ths', m / ths ==> m' / ths').
+Proof.
+  intros * [[Hlen Hmem] Hths].
+  assert (forall i, i < length mt -> i < length m). { rewrite Hlen. trivial. }
+
+  induction Htype; subst; auto using value; right;
+  try match goal with F : lookup empty _ = Some _ |- _ => inversion F end;
+  repeat match goal with
+    IH : _ = empty -> _ |- _ => specialize (IH eq_refl) as [? | [? [? [? ?]]]]
+  end;
+  try solve [eexists; eexists; eexists; eauto using step];
+  repeat match goal with
+    Hv : value ?t , Htype : _ / _ |-- ?t is _ |- _ =>
+      destruct Hv; inversion Htype; subst
+  end;
+  eexists; eexists; eexists; eauto using step, value.
+Qed.
